lib/Digits.dfy
@@ -1,0 +1,57 @@
+include "Seq.dfy"
+include "DivMod.dfy"
+
+module DigitsModule {
+
+  import opened Seq
+  import DivMod
+
+  // Verification of all lemmas is faster with {:opaque}
+  function {:opaque} Digits(n: int, base: int): seq<int> 
+    requires 2 <= base
+  {
+    if n <= 0 then [0] else if n < base then [n] else Digits(n / base, base) + [n % base]
+  }
+
+  lemma DigitsOne(n: int, base: int)
+    requires 2 <= base
+    ensures n < 0 ==> Digits(n, base) == [0]
+    ensures 0 <= n < base ==> Digits(n, base) == [n]
+  {
+    reveal Digits();
+  }
+
+  lemma DigitsBound(n: int, base: int, i: int)
+    requires 2 <= base
+    requires 0 <= i < |Digits(n, base)|
+    ensures 0 <= Digits(n, base)[i] < base
+  {
+    reveal Digits();
+  }
+
+  lemma DigitsSpec(n: int, base: int)
+    requires 0 <= n && 2 <= base
+    ensures Foldl((r, d) => r * base + d, 0, Digits(n, base)) == n
+  {
+    reveal Digits();
+  }
+
+  lemma DigitsSplit(a: int, b: int, base: int)
+    requires 2 <= base
+    requires 0 < a && 0 <= b < base
+    ensures Digits(a * base + b, base) == Digits(a, base) + [b]
+  {
+    DivMod.DivModMulAdd(a, base, b);
+    reveal Digits();
+  }
+
+  lemma DigitsNoLeading0(a: int, base: int)
+    requires 2 <= base
+    requires 0 < a
+    ensures 0 < |Digits(a, base)|
+    ensures 0 < Digits(a, base)[0]
+  {
+    reveal Digits();
+  }
+
+}
